br93

examples/br93.ec
@@ -200,107 +200,9 @@ swap{2} -2.
 save.
 
 
-lemma prob1_1 :
- forall (A <: Adv {M,RO,ARO}),
-(forall (O <: ARO), islossless O.o => islossless A(O).a1) =>
-(forall (O <: ARO), islossless O.o => islossless A(O).a2) =>
- forall &m , Pr[CPA(BR,A).main() @ &m: res] <=
-             Pr[CPA(BR2,A).main() @ &m : res \/ mem M.r ARO.log].
-proof.
- intros A Hlossless1 Hlossless2 &m.
- equiv_deno (_ : (glob A){1} = (glob A){2} ==>
- !(mem M.r ARO.log){2} => res{1} = res{2});
-   [ apply (eq1(A) _ _);try assumption| |];smt.
-save.
-
-
-lemma prob1_2 :
- forall (A <: Adv {M,RO,ARO}),
- forall &m,
-Pr[CPA(BR2,A).main() @ &m : res \/ mem M.r ARO.log] <=
-Pr[CPA(BR2,A).main() @ &m : res ] + 
-Pr[CPA(BR2,A).main() @ &m :  mem M.r ARO.log].
-proof.
- intros A &m.
- cut H:
- (Pr[CPA(BR2,A).main() @ &m : res \/ mem M.r ARO.log] =
-  Pr[CPA(BR2,A).main() @ &m : res] +  Pr[CPA(BR2,A).main() @ &m : mem M.r ARO.log] -
-  Pr[CPA(BR2,A).main() @ &m : res /\ mem M.r ARO.log]).
- pr_or;smt.
- rewrite H.
- cut Hge:(0%r <= (Pr[CPA(BR2,A).main() @ &m : res /\ mem M.r ARO.log])).
- smt.
- generalize Hge.
- generalize (Pr[CPA(BR2,A).main() @ &m : res /\ mem M.r ARO.log]).
- generalize (Pr[CPA(BR2,A).main() @ &m : res]).
- generalize (Pr[CPA(BR2,A).main() @ &m : mem M.r ARO.log]).
- smt.
-save.
-
 lemma real_le_trans : forall(a, b, c : real),  
  Real.(<=) a b => Real.(<=) b  c => a <= c by [].
 
-lemma prob1_3 :
- forall (A <: Adv {M,RO,ARO}),
-(forall (O <: ARO), islossless O.o => islossless A(O).a1) =>
-(forall (O <: ARO), islossless O.o => islossless A(O).a2) =>
- forall &m, Pr[CPA(BR,A).main() @ &m: res] <=
-             Pr[CPA(BR2,A).main() @ &m : res ] + 
-             Pr[CPA(BR2,A).main() @ &m :  mem M.r ARO.log].
-proof.
- intros A Hlossless1 Hlossless2 &m.
- apply (real_le_trans _
-         Pr[CPA(BR2,A).main() @ &m : res \/ mem M.r ARO.log] _ _ _).
- apply (prob1_1 (A) _ _ &m );try assumption;smt.
- apply (prob1_2 (A)  &m).
-save.
-
-(* Step 2: modify the cpa game so the sampling of b is done at the end *)
-
-module CPA2(S : Scheme, A_ : Adv) = {
- module ARO = ARO(RO)
- module A = A_(ARO)
- module SO = S(RO)
-  fun main(): bool = {
-  var pk:pkey;
-  var sk:skey;
-  var m0, m1 : plaintext;
-  var c : ciphertext;
-  var b,b' : bool;
-  ARO.init();
-  (pk,sk)  = SO.kg();
-  (m0,m1)  = A.a1(pk);
-  c  = SO.enc(pk,b?m0:m1);
-  b' = A.a2(c);
-  b = ${0,1}; 
-  return b = b';
- } 
-}.
-
-lemma eq2 : forall (A <: Adv {M,RO,ARO}), 
-(forall (O <: ARO), islossless O.o => islossless A(O).a1) =>
-(forall (O <: ARO), islossless O.o => islossless A(O).a2) =>
- equiv [ CPA(BR2,A).main ~ CPA2(BR2,A).main : 
- (glob A){1} = (glob A){2} ==> ={res,ARO.log,M.r}].
-proof.
- intros A Hlossless1 Hlossless2.
- fun.
- swap{2} -1.
- call (={ARO.log,RO.m,M.r,c} /\ (glob A){1} = (glob A){2})
-      (={ARO.log,RO.m,M.r,res} /\ (glob A){1} = (glob A){2}).
- fun (={ARO.log,RO.m,M.r});[smt|smt|].
- fun;if;[smt|inline RO.o;wp;rnd |];wp;skip;progress;smt.
- inline CPA(BR2, A).SO.enc CPA2(BR2, A).SO.enc.
- swap{2} -3;do 3!(wp;rnd);wp.
- call (={ARO.log,RO.m,p} /\ (glob A){1} = (glob A){2})
-      (={ARO.log,RO.m,res} /\ (glob A){1} = (glob A){2}).
- fun (={ARO.log,RO.m});[smt|smt|].
- fun;if;[smt|inline RO.o;wp;rnd |];wp;skip;progress;smt.
- inline  CPA2(BR2, A).SO.kg CPA2(BR2, A).ARO.init 
-         CPA(BR2, A).SO.kg CPA(BR2, A).ARO.init RO.init.
-admit.
-(* do 2!(wp;);wp;skip;progress;smt. *)
-save.
 
 lemma prob1_1 : 
  forall (A <: Adv {M,RO,ARO}), 
@@ -321,31 +223,29 @@ proof.
  fun;if;[inline RO.o;wp;rnd 1%r (cPtrue)|];wp;skip;smt.
  inline CPA2(BR2,A).SO.kg CPA2(BR2,A).ARO.init RO.init.
  wp;rnd 1%r (cPtrue);wp;skip;progress;[smt|smt|smt|].
- rewrite Dbool.mu_def; case (result);delta charfun;simplify;smt.
+ rewrite Dbool.mu_def.
+ case (result);delta charfun;simplify;smt.
  bdhoare_deno H1; smt.
 save.
 
-lemma prob2_2 : 
- forall (A <: Adv {M,RO,ARO}), 
-(forall (O <: ARO), islossless O.o => islossless A(O).a1) =>
-(forall (O <: ARO), islossless O.o => islossless A(O).a2) =>
- forall &m, Pr[CPA(BR2,A).main() @ &m: res] = Pr[CPA2(BR2,A).main() @ &m : res].
-proof.
- intros A Hlossless1 Hlossless2 &m.
- equiv_deno (_ : (glob A){1} = (glob A){2} ==> ={res,ARO.log,M.r});[|smt|smt].
- apply (eq2(A) _ _); assumption.
-save.
-
-lemma prob2_3 : 
- forall (A <: Adv {M,RO,ARO}), 
+lemma prob1_2 :
+ forall (A <: Adv {M,RO,ARO}) &m,
 (forall (O <: ARO), islossless O.o => islossless A(O).a1) =>
 (forall (O <: ARO), islossless O.o => islossless A(O).a2) =>
 Pr[CPA(BR,A).main() @ &m: res] <=
 1%r/2%r + Pr[CPA2(BR2,A).main() @ &m : mem M.r ARO.log].
 proof.
- intros A Hlossless1 Hlossless2 &m.
- equiv_deno (_ : (glob A){1} = (glob A){2} ==> ={res,ARO.log,M.r});[|smt|smt].
- apply (eq2(A) _ _);assumption.
+ intros A &m Hlossless1 Hlossless2.
+ rewrite -(prob1_1 A _ _ &m);[assumption | assumption | ].
+ apply (real_le_trans _ 
+             Pr[CPA2(BR2,A).main() @ &m : res \/ mem M.r ARO.log] _).
+ equiv_deno (_ : (glob A){1} = (glob A){2} ==>
+ !(mem M.r ARO.log){2} => res{1} = res{2});
+   [ apply (eq1 A _ _);try assumption| |];smt.
+ cut H:
+ (Pr[CPA2(BR2,A).main() @ &m : res \/ mem M.r ARO.log] =
+  Pr[CPA2(BR2,A).main() @ &m : res] +  Pr[CPA2(BR2,A).main() @ &m : mem M.r ARO.log] -
+  Pr[CPA2(BR2,A).main() @ &m : res /\ mem M.r ARO.log]);[pr_or|];smt.
 save.
 
 module type Inverter = {
@@ -452,20 +352,15 @@ lemma Reduction (A <: Adv {M,RO,ARO}) &m :
 Pr[CPA(BR,A).main() @ &m : res] <= 1%r / 2%r + Pr[OW(BR_OW(A)).main() @ &m : res].
 proof.
  intros Hlossless1 Hlossless2.
- apply (real_le_trans _
- (Pr[CPA(BR2,A).main() @ &m : res ] + 
-  Pr[CPA(BR2,A).main() @ &m : mem M.r ARO.log]) _ _ _).
-  apply (prob1_3(A) _ _ &m);try assumption.
-  rewrite (prob2_2(A) _ _ &m);try assumption.
-  rewrite (prob2_3(A) _ _ &m);try assumption.
-  rewrite (prob2_1(A) _ _ &m);try assumption.
-  cut aux: (forall (a b c : real), b <= c => a + b <= a + c).
-  smt.
-  apply (aux (1%r/2%r) (Pr[CPA2(BR2,A).main() @ &m : mem M.r ARO.log])
-  Pr[OW(BR_OW(A)).main() @ &m : res] _).
-  equiv_deno (_ : (glob A){1} = (glob A){2} ==> 
-  mem M.r{1} ARO.log{1} => res{2});[|smt|smt].
-  apply (eq3(A) _ _);assumption.
+ apply (real_le_trans _  
+               (1%r/2%r + Pr[CPA2(BR2,A).main() @ &m : mem M.r ARO.log]) _).
+ apply (prob1_2 A &m _ _ );assumption.
+ cut H: (Pr[CPA2(BR2,A).main() @ &m : mem M.r ARO.log] <=
+         Pr[OW(BR_OW(A)).main() @ &m : res]).
+ equiv_deno (_ : (glob A){1} = (glob A){2} ==>
+ (mem M.r ARO.log){1} => res{2});trivial.
+ apply (eq2 A);assumption.
+ by smt.
 save.
 
 lemma Conclusion (A <: Adv {M,RO,ARO}) &m :
@@ -478,5 +373,5 @@ proof.
  cut aux : 
  (forall (x, y:real), x <= 1%r / 2%r + y => x - 1%r / 2%r  <= y);first smt.
  apply (aux _ _ _).
- apply (Reduction (A) &m _ _);assumption.
+ apply (Reduction A &m _ _);assumption.
 save.
